compiler/backend/proofs/clos_constantProofScript.sml
@@ -32,7 +32,6 @@ End
 Definition parts_def:
   parts (ConstInt i) n aux = make_part n (Int i) aux ∧
   parts (ConstStr s) n aux = make_part n (Str s) aux ∧
-  parts (ConstLbl l) n aux = make_part n (Lbl l) aux ∧
   parts (ConstWord64 w) n aux = make_part n (W64 w) aux ∧
   parts (ConstCons t cs) n aux =
     (let (n, rs, aux) = parts_list cs n aux in
@@ -47,7 +46,6 @@ End
 Definition to_parts_def:
   to_parts (ConstInt i) = [Int i] ∧
   to_parts (ConstStr s) = [Str s] ∧
-  to_parts (ConstLbl l) = [Lbl l] ∧
   to_parts (ConstWord64 w) = [W64 w] ∧
   to_parts (ConstCons t cs) =
     let (n, rs, aux) = parts_list cs 0 [] in
@@ -59,7 +57,6 @@ End
 Definition build_part_def:
   build_part mem (Int i) = ConstInt i ∧
   build_part mem (Str s) = ConstStr s ∧
-  build_part mem (Lbl l) = ConstLbl l ∧
   build_part mem (W64 w) = ConstWord64 w ∧
   build_part mem (Con t ns) = ConstCons t (MAP mem ns)
 End
@@ -206,7 +203,6 @@ Proof
   \\ TRY
    ((rename [‘_ = ConstInt _’] ORELSE
      rename [‘_ = ConstStr _’] ORELSE
-     rename [‘_ = ConstLbl _’] ORELSE
      rename [‘_ = ConstWord64 _’])
     \\ fs [PULL_EXISTS]
     \\ reverse (gvs [make_part_def,AllCaseEqs()])
